Rename old vale-dafny asm procedures

providers/evercrypt/c/evercrypt_vale_stubs.c
@@ -28,37 +28,37 @@ void aes128_encrypt_one_block(uint8_t *out, uint8_t *in, uint8_t *w, uint8_t *sb
 #if !defined(_M_X64) && !defined(__x86_64__)
 /* On non-x64 builds, define no-op stubs for Vale assembly code to avoid */
 /* unresolved symbols while we wait for 32-bit Vale implementations. */
-void __stdcall aes128_key_expansion(uint8_t *key_ptr, uint8_t *expanded_key_ptr)
+void __stdcall old_aes128_key_expansion(uint8_t *key_ptr, uint8_t *expanded_key_ptr)
 {
     KRML_HOST_EPRINTF("Vale aes128_key_expansion() isn't implemented in this platform.  Do not call.\n");
     KRML_HOST_EXIT(255);
 }
 
-void __stdcall gcm128_encrypt_old(void *x0)
+void __stdcall old_gcm128_encrypt(void *x0)
 {
     KRML_HOST_EPRINTF("Vale gcm128_encrypt() isn't implemented in this platform.  Do not call.\n");
     KRML_HOST_EXIT(255);
 }
 
-void __stdcall gcm128_decrypt(void *x0)
+void __stdcall old_gcm128_decrypt(void *x0)
 {
     KRML_HOST_EPRINTF("Vale gcm128_decrypt() isn't implemented in this platform.  Do not call.\n");
     KRML_HOST_EXIT(255);
 }
 
-void __stdcall aes256_key_expansion(uint8_t *key_ptr, uint8_t *expanded_key_ptr)
+void __stdcall old_aes256_key_expansion(uint8_t *key_ptr, uint8_t *expanded_key_ptr)
 {
     KRML_HOST_EPRINTF("Vale aes256_key_expansion() isn't implemented in this platform.  Do not call.\n");
     KRML_HOST_EXIT(255);
 }
 
-void __stdcall gcm256_encrypt_old(void *x0)
+void __stdcall old_gcm256_encrypt(void *x0)
 {
     KRML_HOST_EPRINTF("Vale gcm256_encrypt() isn't implemented in this platform.  Do not call.\n");
     KRML_HOST_EXIT(255);
 }
 
-void __stdcall gcm256_decrypt(void *x0)
+void __stdcall old_gcm256_decrypt(void *x0)
 {
     KRML_HOST_EPRINTF("Vale gcm256_decrypt() isn't implemented in this platform.  Do not call.\n");
     KRML_HOST_EXIT(255);
