providers/evercrypt/EverCrypt.Vale.fsti
@@ -25,19 +25,19 @@ type gcm_args = {
 }
 
 [@ (CCConv "stdcall") ]
-val aes128_key_expansion: key_ptr:uint8_p -> expanded_key_ptr: uint8_p -> Stack_ unit
+val old_aes128_key_expansion: key_ptr:uint8_p -> expanded_key_ptr: uint8_p -> Stack_ unit
 
 [@ (CCConv "stdcall") ]
-val gcm128_encrypt_old: B.pointer gcm_args -> Stack_ unit
+val old_gcm128_encrypt: B.pointer gcm_args -> Stack_ unit
 
 [@ (CCConv "stdcall") ]
-val gcm128_decrypt: B.pointer gcm_args -> Stack_ uint32_t
+val old_gcm128_decrypt: B.pointer gcm_args -> Stack_ uint32_t
 
 [@ (CCConv "stdcall") ]
-val aes256_key_expansion: key_ptr:uint8_p -> expanded_key_ptr: uint8_p -> Stack_ unit
+val old_aes256_key_expansion: key_ptr:uint8_p -> expanded_key_ptr: uint8_p -> Stack_ unit
 
 [@ (CCConv "stdcall") ]
-val gcm256_encrypt_old: B.pointer gcm_args -> Stack_ unit
+val old_gcm256_encrypt: B.pointer gcm_args -> Stack_ unit
 
 [@ (CCConv "stdcall") ]
-val gcm256_decrypt: B.pointer gcm_args -> Stack_ uint32_t
+val old_gcm256_decrypt: B.pointer gcm_args -> Stack_ uint32_t
